proof/correctness768/MLKEM_Poly.ec
@@ -1,7 +1,7 @@
 require import AllCore List IntDiv CoreMap IntDiv Real Number Ring StdOrder.
 
 from Jasmin require import JModel JMemory.
-from JazzEC require import Array32 Array320 Array256 Array128 Array384 Array1024.
+from JazzEC require import Array32 Array320 Array256 Array128 Array384 Array1024 WArray384.
 
 require import IntDiv_extra W16extra.
 
@@ -523,6 +523,9 @@ rewrite -get_to_list  H2 H3 /decompress_poly.
   rewrite modz_small; smt(@Zq).  
 qed.
 
+(********** END BDEP PROOF OF FROMMSG **************)
+
+
 lemma poly_frommsg_corr (_m : W8.t Array32.t): 
     phoare [Jkem768.M._i_poly_frommsg :
              ap =  _m 
@@ -811,13 +814,131 @@ lemma poly_reduce_corr (_a : coeff Array256.t):
           forall k, 0 <= k < 256 => bpos16  res.[k] (2*q)] = 1%r.
 proof. by conseq poly_reduce_ll (poly_reduce_corr_h _a). qed.
 
-lemma poly_tobytes_corr _a : 
+(********** BEGIN BDEP PROOF OF TOBYTES **************)
+
+op tobytes_circuit(a : W16.t) : W12.t = 
+   if (a \ult W16.of_int 3329) then truncateu12 a else truncateu12 (W16_sub a (W16.of_int 3329)).  
+
+module ToBytesInit = {
+    proc toBytesInit(rp: W8.t Array384.t, a: W16.t Array256.t) : W8.t Array384.t *  W16.t Array256.t = {
+       rp <- init_384_8 (fun i => W8.zero);
+       (rp,a) <@ Jkem768.M._poly_tobytes(rp,a);
+       return (rp,a);
+    }
+}.
+
+lemma tobytesinit_ll : islossless ToBytesInit.toBytesInit.
+proc;inline 2.
+wp;while (0 <= i <= 256) (256-i); last by wp; call (poly_csubq_ll); auto =>  /> /#.
+move => *; auto => /> /#.
+qed.
+
+lemma poly_tobytes_ll : islossless Jkem768.M._poly_tobytes.
+proc.
+wp;while (0 <= i <= 257) (257-i); last by wp; call (poly_csubq_ll); auto =>  /> /#.
+move => *; auto => /> /#.
+qed.
+
+lemma poly_tobytes_corr_h _aw : 
     hoare [Jkem768.M._poly_tobytes :
              pos_bound256_cxq a 0 256 2 
-         /\  lift_array256 a = _a
+         /\  _aw = a
               ==>
-             res.`1 = encode12 (map asint _a)].
-admitted.
+             res.`1 = encode12 (map asint (lift_array256 _aw))].
+proof.
+bypr => &m H.
+rewrite Pr[mu_not].
+have -> : Pr[M._poly_tobytes(rp{m}, a{m}) @ &m : true] = 1%r by byphoare => //;apply poly_tobytes_ll.
+have : Pr[M._poly_tobytes(rp{m}, a{m}) @ &m : res.`1 = encode12 (map asint (lift_array256 _aw))] = 1%r; last by smt().
+have <- : Pr[ ToBytesInit.toBytesInit(rp{m}, a{m}) @ &m : res.`1 =  encode12 (map asint (lift_array256 _aw))] = 1%r; last first.
++ byequiv (: ={a} ==> ={res}) => //.
+  proc;inline *.
+  admit.
+
+byphoare (: pos_bound256_cxq a 0 256 2 /\  a = _aw ==> 
+    res.`1 = encode12 (map asint (lift_array256 _aw))) => //.
+conseq tobytesinit_ll (: _  ==> _);1:smt(). 
+proc; inline *.
+proc change ^while.2: (W16_sub t (W16.of_int 3329)); 1: by auto.
+proc change ^while.4 : (sra_16 b (W16.of_int 15)); 1: by auto.
+proc change ^while{2}.7 : (srl_16 t0 (W16.of_int 8)); 1: by auto.
+proc change ^while{2}.10 : (sll_16 d (W16.of_int 4)); 1: by auto.
+proc change ^while{2}.14 : (srl_16 t1 (W16.of_int 4)); 1: by auto.
+proc change ^while{2}.5 : rp0.[j <- truncateu8 d]. admit.
+proc change ^while{2}.12 : rp0.[j <- truncateu8 d]. admit.
+proc change ^while{2}.15 : rp0.[j <- truncateu8 t1]. admit.
+
+unroll for 6.
+unroll for ^while.
+cfold ^i0<-.
+cfold ^i<-.
+cfold ^j<-.
+wp -4.
+bdep 16 12 [_aw] [a] [rp0] tobytes_circuit pcond_reduced. 
+
+(* BDEP pre conseq *)
++ move => &hr />; rewrite flatten1 /= pre_lane_commute_in_aligned 1:/# //=.
+  rewrite allP /pos_bound256_cxq /= => Hb. 
+  rewrite /pcond_reduced /= /tolist /= => x.
+  rewrite  mkseqP => He;elim He => /= i [ib?]; rewrite ultE /=.
+  have := Hb i; rewrite ib /= qE /=.
+  rewrite /to_sint /smod /=.
+  smt(W16.to_uint_cmp).
+
+(* BDEP post conseq *)
+
+(* We start with some boilerplate *)
+move => &hr [#]/= H0 <- rr; rewrite /= !flatten1.
+move => H1; have H2 := post_lane_commute_in_aligned (to_list a{hr}) (to_list rr) W16.w2bits W16.bits2w W8.w2bits W8.bits2w bool2bits bits2bool  compress1_circuit 16 1 8 _ _ _ _ _ _ _ _ _ _ _ _ H1;1..12:
+smt(Array32.size_to_list Array256.size_to_list W16.bits2wK BVA_Top_Pervasive_bool.oflistP).
+
+apply (inj_eq Array32.to_list Array32.to_list_inj).
+apply (flatten_map_eq _ _ W8.w2bits 8 _ W8.w2bits_inj W8.size_w2bits);1:smt().
+have -> := post_lane_commute_in_aligned (to_list a{hr}) (to_list rr) W16.w2bits W16.bits2w W8.w2bits W8.bits2w bool2bits bits2bool  compress1_circuit 16 1 8 _ _ _ _ _ _ _ _ _ _ _ _ H1;1..12:
+    smt(Array32.size_to_list Array256.size_to_list W16.bits2wK BVA_Top_Pervasive_bool.oflistP).
+
+rewrite output_pack_32_8. 
++ rewrite (EclibExtra.size_flatten' 1);1: smt(mapP BS2Int.size_int2bs).
+  by rewrite size_map size_to_list /=.
+
+congr.
+rewrite /compress1_circuit /compress_poly -map_comp -map_comp -map_comp /(\o) /=.  
+apply (eq_from_nth witness); 1: by rewrite !size_map //.
+rewrite size_map size_iota /max /= => i ib; rewrite !(nth_map witness) //=;1,2:smt(size_iota).
+rewrite nth_iota 1:/# -(BVA_Top_Pervasive_bool.oflistP (BS2Int.int2bs 1 (map (compress 1) (lift_array256 a{hr})).[i]));1: by rewrite BS2Int.size_int2bs /#.
+congr; rewrite -BVA_Top_Pervasive_bool.ofintP /lift_array256;rewrite !mapiE;1,2:smt().
+
+rewrite /i2b !get_to_uint /=.
+
+(* This is now the equivalence betwen specs. It's made slightly more verbose
+   because the impl circuit is only proved correct wrt compress for values
+   in the q range. *)
+rewrite ultE /=. 
+case (to_uint a{hr}.[i] < 3329) => /= *.
++ rewrite -compress_impl_small //=;1: by rewrite /bpos16 qE /= /to_sint /smod /=;smt(W16.to_uint_cmp).  
+  congr;congr;rewrite modz_mod;congr;congr.
+  by rewrite /srl_32 /sll_32 /(`<<`) /(`>>`).
+
+have := H0;rewrite /pos_bound256_cxq qE /= => H00.
+
+have ? : 0 <= to_sint ((W16_sub a{hr}.[i] (W16.of_int 3329))) < 3329.
++  rewrite /bpos16 to_sintB_small /=;1: by rewrite  /(to_sint (W16.of_int 3329))  W16.of_uintK /= /smod /=;smt(size_map size_iota). 
+   by rewrite  /(to_sint (W16.of_int 3329))  W16.of_uintK /= /smod /=; smt(size_map size_iota W16.to_uint_cmp).
+
+have ? : to_sint ((W16_sub a{hr}.[i] (W16.of_int 3329))) = to_sint a{hr}.[i] -  3329.
++  rewrite to_sintB_small /=;1: by rewrite  /(to_sint (W16.of_int 3329))  W16.of_uintK /= /smod /=;smt(size_map size_iota). 
+   by rewrite  /(to_sint (W16.of_int 3329))  W16.of_uintK /= /smod /=; smt(size_map size_iota W16.to_uint_cmp).
+
+have -> : (incoeff (to_sint a{hr}.[i])) = (incoeff (to_sint (W16_sub a{hr}.[i] (W16.of_int 3329)))) by  rewrite -eq_incoeff;  smt().  
+
+rewrite -compress_impl_small //=;1:by smt().
+by rewrite modz_mod /srl_32 /sll_32 /(`<<`) /(`>>`).
+qed.
+
+(********** END BDEP PROOF OF TOMSG **************)
+
+
+
 
 lemma poly_frombytes_corr (_a : W8.t Array384.t): 
     hoare [Jkem768.M._poly_frombytes :
